Start defining some predicates on terms.

crypto.v
@@ -8,7 +8,7 @@ From iris.heap_lang Require Import notation proofmode metatheory.
 From iris.heap_lang Require Import primitive_laws.
 From iris.base_logic.lib Require Import invariants.
 From iris_string_ident Require Import ltac2_string_ident.
-From crypto Require Import basic.
+From crypto Require Import basic symbols.
 
 Section Terms.
 
@@ -41,38 +41,85 @@ Class termSG := TermSG {
 
 Context `{termSG}.
 
-Fixpoint lo_opaque s t : iProp Σ :=
+Definition wf_nonce s l : iProp Σ :=
+  symbol1 lo_nonce_name s l ∨
+  symbol1 hi_nonce_name s l.
+Global Instance persistent_wf_nonce s l : Persistent (wf_nonce s l).
+Proof. apply _. Qed.
+
+Definition wf_key s l : iProp Σ :=
+  symbol1 lo_key_name s l ∨
+  symbol1 hi_key_name s l.
+Global Instance persistent_wf_key s l : Persistent (wf_key s l).
+Proof. apply _. Qed.
+
+(* Holds iff all the symbols that appear in the term have been allocated. *)
+Fixpoint wf_term s t : iProp Σ :=
+  match t with
+  | TInt _ => True%I
+  | TPair t1 t2 => wf_term s t1 ∗ wf_term s t2
+  | TNonce l => wf_nonce s l
+  | TKey l => wf_key s l
+  | TEnc l t => wf_key s l ∗ wf_term s t
+  end.
+Global Instance persistent_wf_term s t : Persistent (wf_term s t).
+Proof. elim: t=> /=; apply _. Qed.
+
+(* Opaque terms are those that cannot be inspected by the attacker. *)
+Definition opaque1 s t : iProp Σ :=
   match t with
   | TInt _ => False%I
   | TPair _ _ => False%I
-  | TNonce l => symbol lo_nonce (if s then L l else R l)
+  | TNonce l => symbol1 lo_nonce_name s l
   | TKey l => False%I
-  | TEnc l t => symbol
+  | TEnc l t => symbol1 hi_key_name s l ∗ wf_term s t
   end.
+
+Global Instance persistent_opaque1 s t : Persistent (opaque1 s t).
+Proof. elim: t=> /=; apply _. Qed.
+
+Lemma opaque1_wf_term s t : opaque1 s t -∗ wf_term s t.
+Proof.
+case: t=> /=.
+- by iIntros (_) "?".
+- by iIntros (??) "?".
+- by iIntros (?) "?"; iLeft.
+- by iIntros (?) "?".
+- by iIntros (??) "[??]"; iFrame.
+Qed.
 
 Implicit Types TT : gsetUR (prodO valO valO).
 
 Definition opaque_inv : iProp Σ :=
   ∃ TT, own term_name (● TT)
+        ∗ ⌜perm TT⌝
         ∗ (∀ v1 v2, ⌜(v1, v2) ∈ TT⌝ -∗
            ∃ t1 t2, ⌜v1 = val_of_term t1⌝ ∗
                     ⌜v2 = val_of_term t2⌝ ∗
-                    opaque Left t1 ∗ opaque Right t2).
+                    opaque1 true t1 ∗ opaque1 false t2).
 
-Fixpoint lo_term' t1 t2 : iProp Σ :=
-  own term_name (◯ {[val_of_term t1, val_of_term t2]}) ∨
+Definition opaque v1 v2 : iProp Σ :=
+  own term_name (◯ {[v1, v2]}).
+
+Fixpoint lo_term_aux t1 t2 : iProp Σ :=
+  opaque (val_of_term t1) (val_of_term t2) ∨
   match t1, t2 with
   | TInt n1, TInt n2 => ⌜n1 = n2⌝
   | TPair t11 t12, TPair t21 t22 =>
-    lo_term' t11 t21 ∗ lo_term' t12 t22
+    lo_term_aux t11 t21 ∗ lo_term_aux t12 t22
   | TNonce l1, TNonce l2 =>
-    symbol lo_nonce #l1 #l2
+    symbol lo_nonce_name (LR l1 l2)
   | TKey l1, TKey l2 =>
-    symbol lo_key #l1 #l2
+    symbol lo_key_name (LR l1 l2)
   | TEnc l1 t1, TEnc l2 t2 =>
-    symbol lo_key #l1 #l2 ∗ lo_term' t1 t2
+    symbol lo_key_name (LR l1 l2) ∗ lo_term_aux t1 t2
   | _, _ => False%I
   end.
+
+Definition lo_term v1 v2 : iProp Σ :=
+  ∃ t1 t2, ⌜v1 = val_of_term t1⌝ ∗
+           ⌜v2 = val_of_term t2⌝ ∗
+           lo_term_aux t1 t2.
 
 
 
